Additional instances for TraceMonad to play better with other monad transformers.

src/TraceMonad.v
@@ -4,14 +4,18 @@ Set Implicit Arguments.
 Set Maximal Implicit Arguments.
 
 Class MonadTrace (T : Type) (m : Type -> Type) : Type :=
-{ mlog : T -> m unit
-; mtrace : forall A, T -> A -> m A
-}.
+{ mlog : T -> m unit }.
 
 Require Import ExtLib.Data.Monads.StateMonad.
+Require Import ExtLib.Data.Monads.ReaderMonad.
+Require Import ExtLib.Data.Monads.WriterMonad.
+Require Import ExtLib.Data.Monads.EitherMonad.
 
 Section traceT.
   Variables (T : Type) (m : Type -> Type).
+
+  Import MonadNotation.
+  Local Open Scope monad_scope.
 
   Record traceT (A : Type) := mkTraceT
   { runTraceT : stateT (list T) m A }.
@@ -20,6 +24,9 @@ Section traceT.
     runStateT (runTraceT c) nil.
 
   Context {Monad_m : Monad m}.
+
+  Global Instance MonadTrace_traceT : MonadTrace T traceT :=
+  { mlog := fun x => mkTraceT (modify (fun y => x::y)%list ;; ret tt) }.
 
   Global Instance Monad_traceT : Monad traceT :=
   { ret := fun _ x => mkTraceT (ret x)
@@ -33,6 +40,13 @@ Section traceT.
     : MonadReader S traceT :=
   { ask := lift ask
   ; local := fun f _ c => mkTraceT (local f (runTraceT c))
+  }.
+ 
+  Global Instance MonadWriter_traceT {T M} {MR: @MonadWriter T M m}
+    : @MonadWriter T M traceT :=
+  { tell := fun x => lift (tell x)
+  ; listen := fun _ x => mkTraceT (listen (runTraceT x))
+  ; pass := fun _ x => mkTraceT (pass (runTraceT x))
   }.
 
   Global Instance MonadState_traceT {S} {MS : MonadState S m} 
@@ -53,6 +67,27 @@ Section traceT.
   { mzero := fun _ => lift mzero }.
 
 End traceT.
+
+Section instances.
+  Variables (T : Type) (m : Type -> Type).
+
+  Global Instance MonadTrace_readerT {T S} {MT : MonadTrace T m}
+    : MonadTrace T (readerT S m) :=
+  { mlog := fun x => lift (mlog x) }.
+
+  Global Instance MonadTrace_writerT {T S} {M : Monoid.Monoid S} {MT : MonadTrace T m} (Mo : Monad m)
+    : MonadTrace T (writerT M m) :=
+  { mlog := fun x => @lift (writerT M m) m (MonadT_writerT M Mo) _ (mlog x) }.
+
+  Global Instance MonadTrace_stateT {T S} {MT : MonadTrace T m} {Mo : Monad m}
+    : MonadTrace T (stateT S m) :=
+  { mlog := fun x => lift (mlog x) }.
+
+  Global Instance MonadTrace_eitherT {T S} {MT : MonadTrace T m} {Mo : Monad m}
+    : MonadTrace T (eitherT S m) :=
+  { mlog := fun x => lift (mlog x) }.
+
+End instances.
 
 (*
 Inductive TMsg : Type := 
